@prefix dct: <http://purl.org/dc/terms/> .
@prefix rdf: <http://www.w3.org/1999/02/22-rdf-syntax-ns#> .
@prefix skos: <http://www.w3.org/2004/02/skos/core#> .
@prefix xsd: <http://www.w3.org/2001/XMLSchema#> .

<http://openml.org/openml/task-type> a skos:ConceptScheme;
  dct:description "The type of task used to group tasks";
  dct:title "Task type";
  skos:hasTopConcept <http://openml.org/openml/task-type#clustering>, <http://openml.org/openml/task-type#learningcurve>,
    <http://openml.org/openml/task-type#machinelearningchallenge>, <http://openml.org/openml/task-type#subgroupdiscovery>,
    <http://openml.org/openml/task-type#supervisedclassification>, <http://openml.org/openml/task-type#superviseddatastreamclassification>,
    <http://openml.org/openml/task-type#supervisedregression>, <http://openml.org/openml/task-type#survivalanalysis> .

<http://openml.org/openml/task-type#subgroupdiscovery> a skos:Concept;
  dct:identifier "8";
  skos:definition "TBA"@en;
  skos:inScheme <http://openml.org/openml/task-type>;
  skos:prefLabel "Subgroup Discovery"@en;
  skos:topConceptOf <http://openml.org/openml/task-type> .

<http://openml.org/openml/task-type#survivalanalysis> a skos:Concept;
  dct:identifier "7";
  skos:definition "Related to Regression. Given a dataset (typically consisting of patient data) predict a left timestamp (date entering the study), right timestamp (date of leaving the study), or both."@en;
  skos:inScheme <http://openml.org/openml/task-type>;
  skos:prefLabel "Survival Analysis"@en;
  skos:topConceptOf <http://openml.org/openml/task-type> .

<http://openml.org/openml/task-type#machinelearningchallenge> a skos:Concept;
  dct:identifier "6";
  skos:definition "This is a standard machine learning challenge with a hidden private dataset."@en;
  skos:inScheme <http://openml.org/openml/task-type>;
  skos:prefLabel "Machine Learning Challenge"@en;
  skos:topConceptOf <http://openml.org/openml/task-type> .

<http://openml.org/openml/task-type#clustering> a skos:Concept;
  dct:identifier "5";
  skos:definition "Given an input dataset, the task is to partition it into various clusters."@en;
  skos:inScheme <http://openml.org/openml/task-type>;
  skos:prefLabel "Clustering"@en;
  skos:topConceptOf <http://openml.org/openml/task-type> .

<http://openml.org/openml/task-type#superviseddatastreamclassification> a skos:Concept;
  dct:identifier "4";
  skos:definition "Given a dataset with a nominal target, various data samples of increasing size are defined. A model is build for each individual data sample; from this a learning curve can be drawn."@en;
  skos:inScheme <http://openml.org/openml/task-type>;
  skos:prefLabel "Supervised Data Stream Classification"@en;
  skos:topConceptOf <http://openml.org/openml/task-type> .

<http://openml.org/openml/task-type#learningcurve> a skos:Concept;
  dct:identifier "3";
  skos:definition "Given a dataset with a nominal target, various data samples of increasing size are defined. A model is build for each individual data sample; from this a learning curve can be drawn."@en;
  skos:inScheme <http://openml.org/openml/task-type>;
  skos:prefLabel "Learning Curve"@en;
  skos:topConceptOf <http://openml.org/openml/task-type> .

<http://openml.org/openml/task-type#supervisedregression> a skos:Concept;
  dct:identifier "2";
  skos:definition "Given a dataset with a numeric target and a set of train/test splits, e.g. generated by a cross-validation procedure, train a model and return the predictions of that model."@en;
  skos:inScheme <http://openml.org/openml/task-type>;
  skos:prefLabel "Supervised Regression"@en;
  skos:topConceptOf <http://openml.org/openml/task-type> .

<http://openml.org/openml/task-type#supervisedclassification> a skos:Concept;
  dct:identifier "1";
  skos:definition "In supervised classification, you are given an input dataset in which instances are labeled with a certain class. The goal is to build a model that predicts the class for future unlabeled instances. The model is evaluated using a train-test procedure, e.g. cross-validation."@en;
  skos:inScheme <http://openml.org/openml/task-type>;
  skos:prefLabel "Supervised Classification"@en;
  skos:topConceptOf <http://openml.org/openml/task-type> .